ironfleet/src/Dafny/Distributed/Protocol/RSL/FailureProof/Phase2Proof_toplevel.i.dfy
@@ -8,20 +8,25 @@ import opened Rs2Phase2Proof_Helper
 
 
 lemma PerfInvariantMaintained(s:TimestampedRslState, s':TimestampedRslState, req_time:Timestamp, opn:OperationNumber)
-    requires RslAssumption(s) && RslConsistency(s)
-    requires RslAssumption(s') && RslConsistency(s')
+    requires RslAssumption(s) && RslAssumption(s')
+    requires RslConsistency(s) && RslConsistency(s')
     requires TimestampedRslNext(s, s')
     requires RslPerfInvariant(s, opn)
     ensures RslPerfInvariant(s', opn)
 {   
     PacketsBallotInvariant_Maintained(s, s', opn);
+    AlwaysInvariant_Maintained(s, s', opn);
+    
+    if !exists pkt :: pkt in s.t_environment.sentPackets && IsNew2aPacket(pkt, opn) {
+        Before2a_to_BeforeOrAfter2a(s, s', opn);
+    }
+
+    assert AlwaysInvariant(s');        
     assert PacketsBallotInvariant(s');
     
-    PerformanceGuarantee_2a_Maintained(s, s', opn);
-    assert PerformanceGuarantee_2a(s', opn);
-    
     assume false;
-    assert PerformanceGuarantee(s', opn);
+    assert PerformanceGuarantee(s', opn);   // TODO
+    assert RslPerfInvariant(s', opn);
 }
 
 
@@ -30,8 +35,8 @@ lemma PerfInvariantMaintained(s:TimestampedRslState, s':TimestampedRslState, req
 *****************************************************************************************/
 
 lemma PacketsBallotInvariant_Maintained(ts:TimestampedRslState, ts':TimestampedRslState, opn:OperationNumber) 
-    requires RslAssumption(ts) && RslConsistency(ts)
-    requires RslAssumption(ts') && RslConsistency(ts')
+    requires RslAssumption(ts) && RslAssumption(ts')
+    requires RslConsistency(ts') && RslConsistency(ts')
     requires TimestampedRslNext(ts, ts')
     requires RslPerfInvariant(ts, opn)
     ensures PacketsBallotInvariant(ts')
@@ -49,37 +54,51 @@ lemma PacketsBallotInvariant_Maintained(ts:TimestampedRslState, ts':TimestampedR
     }
 }
 
-lemma PerformanceGuarantee_2a_Maintained(ts:TimestampedRslState, ts':TimestampedRslState, opn:OperationNumber) 
+
+lemma Before2a_to_BeforeOrAfter2a(ts:TimestampedRslState, ts':TimestampedRslState, opn:OperationNumber) 
     requires RslAssumption(ts) && RslConsistency(ts)
     requires RslAssumption(ts') && RslConsistency(ts')
     requires PacketsBallotInvariant(ts) && PacketsBallotInvariant(ts')
     requires TimestampedRslNext(ts, ts')
     requires RslPerfInvariant(ts, opn)
-    ensures PerformanceGuarantee_2a(ts', opn);
+    ensures Before_2a_Sent_Invariant(ts', opn) || After_2a_Sent_Invariant(ts', opn);
 {
+    assume false;
     if TimestampedRslNextEnvironment(ts, ts') {
         assert PerformanceGuarantee_2a(ts', opn);
         return;
     }
-    if exists pkt :: pkt in ts.t_environment.sentPackets && IsNew2aPacket(pkt, opn) {
-        /* TODO: I can't say anything about leader timestamp at this point.
-        Leader could send new 2a's out. And these 2a's will be unbounded
-        */
 
-        forall pkt | pkt in ts'.undeliveredPackets && IsNew2aPacket(pkt, opn)
-        ensures TimeLe(pkt.msg.ts, TimeBound2aDeliveryPost())
-        {}
-        assert PerformanceGuarantee_2a(ts', opn);
-        return;
-    }
-    
     var idx, tios:seq<TimestampedLIoOp<NodeIdentity, RslMessage>> :| TimestampedRslNextOneReplica(ts, ts', idx, tios);
+    var nextActionIndex := ts.t_replicas[idx].v.nextActionIndex;
     if idx != 1 {
         assert PerformanceGuarantee_2a(ts', opn);
         return;
     }
+    // Actor is the leader now
+    if exists pkt :: pkt in ts.t_environment.sentPackets && IsNew2aPacket(pkt, opn) {
+        /* TODO: If I enter this clause, then any new 2a packets I sent out can't be of opn */
+
+        if nextActionIndex == 3 {
+            assert PerformanceGuarantee_2a(ts', opn);
+        } else {
+            forall pkt | pkt in ts'.undeliveredPackets && IsNew2aPacket(pkt, opn)
+            ensures pkt in ts.undeliveredPackets
+            {}
+            assert PerformanceGuarantee_2a(ts', opn);
+        }   
+
+
+
+        // forall pkt | pkt in ts'.undeliveredPackets && IsNew2aPacket(pkt, opn)
+        // ensures TimeLe(pkt.msg.ts, TimeBound2aDeliveryPost())
+        // {}
+        // assert PerformanceGuarantee_2a(ts', opn);
+        return;
+    }
     
-    var nextActionIndex := ts.t_replicas[idx].v.nextActionIndex;
+    
+    
     assert nextActionIndex == 3;
     assert PerformanceGuarantee_2a(ts', opn);
 }
